Updating CompCert_new

compcert_new/lib/Coqlib.v
@@ -1332,3 +1332,59 @@ Lemma nlist_forall2_imply:
 Proof.
   induction 1; simpl; intros; constructor; auto.
 Qed.
+
+
+
+Inductive not_empty {A}: list A -> Prop:=
+| not_empty_intros: forall s ls, not_empty (s::ls).
+Lemma nil_not_empty:
+      forall A, @not_empty A nil -> False.
+Proof. intros * H; inv H. Qed.
+Hint Resolve not_empty_intros.
+
+
+
+Inductive list_forall2_end {A B : Type} (P : A -> B -> Prop)
+          (END : A -> B -> Prop): list A -> list B -> Prop :=
+    list_forall2_one: forall a b, END a b -> list_forall2_end P END (a::nil) (b::nil)
+  | list_forall2_end_cons : forall (a1 : A) (al : list A) (b1 : B) (bl : list B),
+                        P a1 b1 ->
+                        list_forall2_end P END al bl ->
+                        list_forall2_end P END (a1 :: al) (b1 :: bl).
+
+
+(* New tactics added by Santiago Cuellar: *)
+(*Do case analysis to simplify a match _ with*)
+Ltac common_tacs_after_destruct H:=
+  first [ congruence
+        | solve[inversion H]
+        | auto].
+      
+Ltac match_case_goal:=
+  match goal with
+    |- context[match ?x with _ => _ end] =>
+    destruct x eqn:?; try congruence
+  end.
+Ltac match_case_hyp H:=
+  match type of H with
+    context[match ?x with _ => _ end] => destruct x eqn:?
+  end; common_tacs_after_destruct H.
+Tactic Notation "match_case":= match_case_goal.
+Tactic Notation "match_case" "in" hyp(H):= (match_case_hyp H).
+
+Ltac split_hyp:=
+  match goal with [H: _ /\ _ |- _ ]=> destruct H end.
+Ltac hard_split:= match goal with [ |- _ /\ _ ]=> split end.
+Lemma ex_impl:
+      forall {A} (P P':A->Prop),  (forall x, P x -> P' x) ->
+                         (exists x, P x) -> (exists x, P' x).
+Proof. intros * ? [].  eexists; eauto. Qed.
+Lemma and_impl:
+  forall (P P' Q: Prop), (P -> P') -> (P /\ Q) -> (P' /\ Q).
+Proof. tauto. Qed.
+(* removes statements from inside existentials and conjunctions *)
+Ltac solve_inside HH:= try solve[eauto];
+  try solve [eapply and_impl; [| solve[eapply HH; eauto]]; simpl;
+       let HH':=fresh in intros HH'; solve_inside HH' ];
+  try solve [eapply ex_impl; [| solve[eapply HH; eauto]]; simpl;
+       let HH':=fresh in intros ? HH'; solve_inside HH'].
